PAC_Checker_LLVM/LPAC_Error.thy
@@ -113,4 +113,106 @@ lemma check_extension_l2_side_cond_err_fref:
 lemmas check_extension_l2_side_cond_err_hnr[sepref_fr_rules] =
   check_extension_l2_side_cond_err_impl.refine[FCOMP check_extension_l2_side_cond_err_fref]
 
+definition check_linear_combi_l_pre_err_imp_s  where
+  \<open>check_linear_combi_l_pre_err_imp_s i pd p mem =
+    (if pd then cl_to_clt ''The polynomial with id '' @ show_nat i 
+              @ cl_to_clt '' was not found'' else cl_to_clt '''') @
+    (if p then cl_to_clt ''The co-factor from '' @ show_nat i 
+              @ cl_to_clt '' was empty'' else cl_to_clt '''') @
+    (if mem then cl_to_clt ''Memory out or new variable'' else cl_to_clt '''')\<close>
+
+sepref_def check_linear_combi_l_pre_err_s_impl
+  is \<open>uncurry3 (RETURN oooo check_linear_combi_l_pre_err_imp_s)\<close>
+  :: \<open>si64_assn\<^sup>k *\<^sub>a bool1_assn\<^sup>k *\<^sub>a bool1_assn\<^sup>k *\<^sub>a bool1_assn\<^sup>k \<rightarrow>\<^sub>a strlt_assn\<close>
+  unfolding check_linear_combi_l_pre_err_imp_s_def
+  by sepref
+
+type_synonym sllist_polynomial = \<open>(nat list \<times> int) list\<close>
+
+abbreviation monom_s_rel where
+  \<open>monom_s_rel \<equiv> \<langle>nat_rel\<rangle>list_rel\<close>
+
+abbreviation monom_s_assn where
+  \<open>monom_s_assn \<equiv> cl_assn' si64_assn\<close>
+
+abbreviation poly_s_assn where
+  \<open>poly_s_assn \<equiv> cl_assn' (monom_s_assn \<times>\<^sub>a sbi_assn)\<close>
+
+definition check_linear_combi_l_s_dom_err :: \<open>sllist_polynomial \<Rightarrow> nat \<Rightarrow> string nres\<close> where
+  \<open>check_linear_combi_l_s_dom_err p r = SPEC (\<lambda>_. True)\<close>
+
+definition check_linear_combi_l_s_dom_err_imp  where
+  \<open>check_linear_combi_l_s_dom_err_imp x p =
+    cl_to_clt ''Poly not found in CL from x '' @ show_nat p\<close>
+
+sepref_def check_linear_combi_l_s_dom_err_impl is
+  \<open>uncurry (RETURN oo check_linear_combi_l_s_dom_err_imp)\<close>
+  :: \<open>poly_s_assn\<^sup>k *\<^sub>a si64_assn\<^sup>k \<rightarrow>\<^sub>a strlt_assn\<close>
+  unfolding check_linear_combi_l_s_dom_err_imp_def
+  by sepref
+
+lemma check_linear_combi_l_s_dom_err_fref:
+  \<open>(uncurry (RETURN oo (check_linear_combi_l_s_dom_err_imp)),
+    uncurry (check_linear_combi_l_s_dom_err)) 
+   \<in> Id \<rightarrow>\<^sub>f \<langle>Id\<rangle>nres_rel\<close>
+  apply (intro frefI nres_relI)
+  unfolding check_linear_combi_l_s_dom_err_imp_def
+    check_linear_combi_l_s_dom_err_def
+  by auto
+
+lemmas check_linear_combi_l_s_dom_err_hnr[sepref_fr_rules] =
+  check_linear_combi_l_s_dom_err_impl.refine[FCOMP check_linear_combi_l_s_dom_err_fref]
+
+(* TODO - need a way to print sllist_polynomial 
+definition check_linear_combi_l_s_mult_err_impl :: \<open>_ \<Rightarrow> _ \<Rightarrow> _\<close>  where
+  \<open>check_linear_combi_l_s_mult_err_impl x p =
+  ''Unequal polynom found in CL '' @ show (map (\<lambda>(a,b). (map nat_of_uint64 a, b)) p) @
+  '' but '' @ show (map (\<lambda>(a,b). (map nat_of_uint64 a, b)) x)\<close>
+
+lemma [sepref_fr_rules]:
+  \<open>(uncurry (return oo (check_linear_combi_l_s_mult_err_impl)),
+    uncurry (check_linear_combi_l_s_mult_err)) \<in> poly_s_assn\<^sup>k *\<^sub>a poly_s_assn\<^sup>k \<rightarrow>\<^sub>a raw_string_assn\<close>
+   unfolding check_linear_combi_l_s_mult_err_impl_def check_linear_combi_l_s_mult_err_def list_assn_pure_conv
+   apply sepref_to_hoare
+   apply sep_auto
+   done
+
+definition check_extension_l_s_new_var_multiple_err_impl :: \<open>String.literal \<Rightarrow> _ \<Rightarrow> _\<close>  where
+  \<open>check_extension_l_s_new_var_multiple_err_impl x p =
+  ''Variable already defined '' @ show x @
+  '' but '' @ show (map (\<lambda>(a,b). (map nat_of_uint64 a, b)) p)\<close>
+
+lemma [sepref_fr_rules]:
+  \<open>(uncurry (return oo (check_extension_l_s_new_var_multiple_err_impl)),
+    uncurry (check_extension_l_s_new_var_multiple_err)) \<in> string_assn\<^sup>k *\<^sub>a poly_s_assn\<^sup>k \<rightarrow>\<^sub>a raw_string_assn\<close>
+   unfolding check_extension_l_s_new_var_multiple_err_impl_def check_extension_l_s_new_var_multiple_err_def list_assn_pure_conv
+   apply sepref_to_hoare
+   apply sep_auto
+   done
+
+definition check_extension_l_s_side_cond_err_impl :: \<open>String.literal \<Rightarrow> _ \<Rightarrow> _\<close>  where
+  \<open>check_extension_l_s_side_cond_err_impl x p p' q' =
+  ''p^2- p != 0 '' @ show x @
+  '' but '' @ show (map (\<lambda>(a,b). (map nat_of_uint64 a, b)) p) @
+  '' and '' @ show (map (\<lambda>(a,b). (map nat_of_uint64 a, b)) p') @
+   '' and ''  @ show (map (\<lambda>(a,b). (map nat_of_uint64 a, b)) q')\<close>
+
+lemma [sepref_fr_rules]:
+  \<open>(uncurry3 (return oooo (check_extension_l_s_side_cond_err_impl)),
+    uncurry3 (check_extension_l_s_side_cond_err)) \<in> string_assn\<^sup>k *\<^sub>a poly_s_assn\<^sup>k*\<^sub>a poly_s_assn\<^sup>k*\<^sub>a poly_s_assn\<^sup>k \<rightarrow>\<^sub>a raw_string_assn\<close>
+   unfolding check_extension_l_s_side_cond_err_impl_def check_extension_l_s_side_cond_err_def list_assn_pure_conv
+   apply sepref_to_hoare
+   apply sep_auto
+   done
+
+*)
+
+definition memory_out_msg where
+  \<open>memory_out_msg = cl_to_clt ''memory out''\<close>
+
+sepref_def memory_out_msg_impl is \<open>uncurry0 (RETURN memory_out_msg)\<close>
+  :: \<open>unit_assn\<^sup>k \<rightarrow>\<^sub>a strlt_assn\<close>
+  unfolding memory_out_msg_def
+  by sepref
+
 end
